dw/Custom/Map.v
@@ -1,0 +1,62 @@
+(* Total maps *)
+
+(* This module is meant to be [Require]-d but not [Import]-ed. *)
+
+From QuickChick Require Import Decidability.
+
+Section Map.
+
+Variable K V : Type.
+Context `{Eq K}.
+
+Definition t : Type := K -> V.
+
+Definition update : K -> V -> t -> t :=
+  fun k0 v0 f k => if k = k0 ? then v0 else f k.
+
+Definition lookup : t -> K -> V := fun f => f.
+
+Lemma update_lookup_eq k k' v m :
+  k = k' ->
+  lookup (update k v m) k' = v.
+Proof.
+  intro Hk.
+  unfold lookup.
+  unfold update.
+  destruct dec.
+  - auto.
+  - subst; contradiction.
+Qed.
+
+Lemma update_lookup_neq k k' v m :
+  k <> k' ->
+  lookup (update k v m) k' = lookup m k'.
+Proof.
+  intros Hk.
+  unfold lookup.
+  unfold update.
+  destruct dec.
+  - subst; contradiction.
+  - auto.
+Qed.
+
+Lemma update_update_eq k k' v v' m :
+  k = k' ->
+  update k v (update k' v' m) = update k v m.
+Proof.
+(* Extensionally... *)
+Admitted.
+
+Lemma lookup_update_eq k k' v m :
+  k = k' ->
+  v = lookup m k' ->
+  update k v m = m.
+Proof.
+(* Also extensional... *)
+Admitted.
+
+End Map.
+
+Arguments t K V : assert.
+Arguments update {K V _}.
+Arguments lookup {K V}.
