dw/DeepWeb/Lib/SimpleSpec_NetworkModel.v
@@ -1,0 +1,212 @@
+(* A model of the network. *)
+
+From Custom Require Import
+     List Map.
+Import ListNotations.
+
+From DeepWeb Require Import
+     Lib.Util.
+
+Module Type NetworkModelInterface.
+
+(* The complete state of the network. *)
+Parameter network_state : Type.
+
+(* The initial state. *)
+Parameter initial_ns : network_state.
+
+(* State transitions.
+   - The result is [None] when a transition is not defined.
+   - Transitions may carry some output (in this case, a byte
+     for [recv] transitions. *)
+Definition transition (output : Type) : Type :=
+  network_state -> option (network_state * output).
+
+(* Server-side transitions *)
+Parameter server_accept : connection_id -> transition unit.
+Parameter server_send : connection_id -> byte -> transition unit.
+Parameter server_recv : connection_id -> transition byte.
+
+(* Client-side transitions *)
+Parameter client_connect : connection_id -> transition unit.
+Parameter client_send : connection_id -> byte -> transition unit.
+Parameter client_recv : connection_id -> transition byte.
+
+End NetworkModelInterface.
+
+Module Export NetworkModel <: NetworkModelInterface.
+
+(* The network state is a map from [connection_id]
+   to the state of the connection ([connection_state]). *)
+
+(* We start by defining the state of a single connection. *)
+
+(* - Connections start in the [CLOSED] state.
+   - When a client initiates a connection ([client_connect]),
+     the connection enters the [PENDING] state, and the client can
+     immediately start sending messages over it.
+   - The server must then accept the connection, which enters
+     the [ACCEPTED] state, before receiving and sending messages
+     over it. The client can now also receive messages.
+ *)
+Inductive connection_state_enum := CLOSED | PENDING | ACCEPTED.
+
+(* A connection can be seen as a pair of buffers. *)
+Record connection_state :=
+  Build_connection_state {
+
+    (* The state of the connection (see above). *)
+    connection_status : connection_state_enum;
+
+    (* The buffer of bytes going into the server. *)
+    connection_inbytes : list byte;
+
+    (* The buffer of bytes going out from the server. *)
+    connection_outbytes : list byte;
+  }.
+
+(* Connections start [CLOSED]. *)
+(* "cs" for [connection_state]. *)
+Definition initial_cs : connection_state := {|
+    connection_status := CLOSED;
+    connection_inbytes := [];
+    connection_outbytes := [];
+  |}.
+
+(* A client-side "connect" updates the connection from [CLOSED]
+   to [PENDING]. *)
+Definition pending_cs : connection_state := {|
+    connection_status := PENDING;
+    connection_inbytes := [];
+    connection_outbytes := [];
+  |}.
+
+(* A server-side "accept" updates the connection from [PENDING]
+   to [ACCEPTED]. There may already be bytes going into the
+   server that we must preserve. *)
+Definition accept_cs (cs : connection_state) : connection_state := {|
+    connection_status := ACCEPTED;
+    connection_inbytes := connection_inbytes cs;
+    connection_outbytes := [];
+  |}.
+
+(* A client sends a byte to the server on some connection by
+   adding it to the connection's "in"-buffer. *)
+Definition update_in (bs : list byte) (cs : connection_state) :
+  connection_state := {|
+    connection_status := connection_status cs;
+    connection_inbytes := bs;
+    connection_outbytes := connection_outbytes cs;
+  |}.
+
+(* A server sends a byte to the client by adding it to the
+   connection's "out"-buffer. *)
+Definition update_out (bs : list byte) (cs : connection_state) :
+  connection_state := {|
+    connection_status := connection_status cs;
+    connection_inbytes := connection_inbytes cs;
+    connection_outbytes := bs;
+  |}.
+
+(* We can now define the complete state of the network. *)
+Definition network_state := Map.t connection_id connection_state.
+
+(* Initial state. *)
+(* "ns" for [network_state]. *)
+Definition initial_ns : network_state := fun _ => initial_cs.
+
+(* State transitions (see [NetworkModelInterface]). *)
+Definition transition (output : Type) : Type :=
+  network_state -> option (network_state * output).
+
+(* The client opens a new connection.
+   The result is [Some] if and only if the connection is [CLOSED],
+   and it then moves to the [PENDING] state, waiting to be accepted
+   by the server. *)
+Definition client_connect (c : connection_id) : transition unit :=
+  fun (ns : network_state) =>
+    let cs := Map.lookup ns c in
+    match connection_status cs with
+    | CLOSED => Some (Map.update c pending_cs ns, tt)
+    | PENDING | ACCEPTED => None
+    end.
+
+Lemma connect_success ns c :
+  connection_status (Map.lookup ns c) = CLOSED ->
+  client_connect c ns = Some (Map.update c pending_cs ns, tt).
+Proof.
+  intro Hc.
+  unfold client_connect.
+  rewrite Hc; auto.
+Qed.
+
+(* The server accepts a [PENDING] connection.
+   The result is [Some] if and only if the connection is [PENDING],
+   and it then moves to the [ACCEPTED] state, indicating that the
+   server can send and recv messages on it. *)
+Definition server_accept (c : connection_id) : transition unit :=
+  fun ns =>
+    let cs := Map.lookup ns c in
+    match connection_status cs with
+    | PENDING => Some (Map.update c (accept_cs cs) ns, tt)
+    | ACCEPTED | CLOSED => None
+    end.
+
+Lemma accept_success ns c :
+  let cs := Map.lookup ns c in
+  connection_status cs = PENDING ->
+  server_accept c ns = Some (Map.update c (accept_cs cs) ns, tt).
+Proof.
+  simpl; intro Hc.
+  unfold server_accept.
+  rewrite Hc; auto.
+Qed.
+
+(* The server receives a byte on a connection.
+   The connection is assumed to be [ACCEPTED], and the result
+   is [Some] if and only if there is a nonempty
+   [connection_inbytes] buffer. *)
+Definition server_recv (c : connection_id) : transition byte :=
+  fun ns =>
+    let cs := Map.lookup ns c in
+    match connection_inbytes cs with
+    | [] => None
+    | b :: bs =>
+      let cs := update_in bs cs in
+      let ns := Map.update c cs ns in
+      Some (ns, b)
+    end.
+
+(* The server sends a byte.
+   The connection is assumed to be [ACCEPTED]. *)
+Definition server_send
+           (c : connection_id) (b : byte) : transition unit :=
+  fun ns =>
+    let cs := Map.lookup ns c in
+    let cs := update_out (connection_outbytes cs ++ [b]) cs in
+    Some (Map.update c cs ns, tt).
+
+(* The client receives a byte sent by the server.
+   The connection is assumed to be [PENDING] or [ACCEPTED]. *)
+Definition client_recv (c : connection_id) : transition byte :=
+  fun ns =>
+    let cs := Map.lookup ns c in
+    match connection_outbytes cs with
+    | [] => None
+    | b :: bs =>
+      let cs := update_out bs cs in
+      let ns := Map.update c cs ns in
+      Some (ns, b)
+    end.
+
+(* The client sends a byte to the server.
+   The connection is assumed to be [ACCEPTED] (the server must
+   accept a connection before sending bytes on it). *)
+Definition client_send
+           (c : connection_id) (b : byte) : transition unit :=
+  fun ns =>
+    let cs := Map.lookup ns c in
+    let cs := update_in (connection_inbytes cs ++ [b]) cs in
+    Some (Map.update c cs ns, tt).
+
+End NetworkModel.
