dw/DeepWeb/Lib/SimpleSpec_Refinement.v
@@ -1,0 +1,76 @@
+Require Import Relations.
+Require Import RelationClasses.
+
+From QuickChick Require Import QuickChick.
+From Custom Require Import List.
+Import ListNotations.
+From Custom Require Map.
+
+Require Import DeepWeb.Free.Monad.Free.
+Require Import DeepWeb.Free.Monad.Common.
+Import NonDeterminismBis.
+Import SumNotations.
+
+Require Import DeepWeb.Lib.Util.
+
+From DeepWeb Require Import
+     Lib.SimpleSpec_NetworkModel
+     Lib.SimpleSpec_NetworkInterface
+     Lib.SimpleSpec_Observer
+     Lib.SimpleSpec_Scramble
+     Lib.SimpleSpec_Traces.
+
+Set Bullet Behavior "Strict Subproofs".
+
+Module MkScramblingRefinement (ScramblingFacts : ScramblingTypes).
+
+Import ScramblingFacts.
+
+Definition refines_mod_network server spec : Prop :=
+  forall tr : real_trace,
+    wf_trace tr ->
+    is_server_trace server tr ->
+    forall str : real_trace,
+      network_scrambled0 tr str ->
+      exists dstr : real_trace,
+        network_scrambled0 dstr str /\
+        is_spec_trace spec dstr.
+
+Definition strong_refines_mod_network server spec : Prop :=
+  forall tr : real_trace,
+    wf_trace tr ->
+    is_server_trace server tr ->
+      exists dstr : real_trace,
+        network_scrambled0 dstr tr /\
+        is_spec_trace spec dstr.
+
+Definition strong_sound :
+  forall server spec,
+    strong_refines_mod_network server spec ->
+    refines_mod_network server spec.
+Proof.
+  intros server spec Hstrong tr Htr_wf Htr_istrace str Hstr_scrambled.
+  destruct (Hstrong tr Htr_wf Htr_istrace)
+    as [dstr [Hdstr_scrambled Hdstr_istrace]].
+  exists dstr.
+  split; auto.
+  etransitivity; eauto.
+Qed.
+
+Definition strong_complete :
+  forall server spec,
+    refines_mod_network server spec ->
+    strong_refines_mod_network server spec.
+Proof.
+  intros server spec Hcorrect tr Htr_wf Htr_istrace.
+  destruct (Hcorrect tr Htr_wf Htr_istrace tr)
+    as [dstr [Hdstr_scrambled Hdstr_istrace]].
+  { apply scrambled_reflexive; auto. }
+  exists dstr.
+  auto.
+Qed.
+
+End MkScramblingRefinement.
+
+Module Export ScramblingRefinement :=
+  MkScramblingRefinement ScramblingFacts.
