dw/DeepWeb/Lib/SimpleSpec_Scramble.v
@@ -1,0 +1,359 @@
+Require Import Relations.
+Require Import RelationClasses.
+
+From QuickChick Require Import QuickChick.
+From Custom Require Import List.
+Import ListNotations.
+From Custom Require Map.
+
+Require Import DeepWeb.Free.Monad.Free.
+Require Import DeepWeb.Free.Monad.Common.
+Import NonDeterminismBis.
+Import SumNotations.
+
+Require Import DeepWeb.Lib.Util.
+
+From DeepWeb Require Import
+     Lib.SimpleSpec_NetworkModel
+     Lib.SimpleSpec_Traces.
+
+Set Bullet Behavior "Strict Subproofs".
+
+Module Type ScramblingTypes.
+
+Parameter wf_trace : forall {byte'}, list (event byte') -> Prop.
+
+Definition network_scrambled_wf ns (tr0 tr1 : real_trace) :=
+  wf_trace tr0 ->
+  wf_trace tr1 ->
+  network_scrambled ns tr0 tr1.
+
+Definition network_scrambled_wf0 := network_scrambled_wf initial_ns.
+
+Declare Instance scrambled_transitive : Transitive network_scrambled0.
+
+Declare Instance scrambled_reflexive : Reflexive network_scrambled_wf0.
+
+End ScramblingTypes.
+
+Module ScramblingFacts <: ScramblingTypes.
+
+Definition project_trace_on {byte'} (c : connection_id) :
+  list (event byte') -> list (event byte') :=
+  filter (fun ev => event_connection ev = c ?).
+
+Definition is_ToFromServer {byte'} (ev : event byte') : bool :=
+  match ev with
+  | NewConnection _ => false
+  | ToServer _ _ | FromServer _ _ => true
+  end.
+
+Definition wf_projection {byte'} (tr : list (event byte')) : bool :=
+  match tr with
+  | [] => true
+  | NewConnection _ :: tr' =>
+    forallb is_ToFromServer tr'
+  | (ToServer _ _ | FromServer _ _) :: _ => false
+  end.
+
+Definition wf_trace {byte'} (tr : list (event byte')) : Prop :=
+  forall c,
+    is_true (wf_projection (project_trace_on c tr)).
+
+Fixpoint open_trace {byte'}
+         (is_open : connection_id -> Prop) (tr : list (event byte')) :
+  Prop :=
+  match tr with
+  | [] => True
+  | NewConnection c :: tr =>
+    ~is_open c /\ open_trace (fun c' => c = c' \/ is_open c') tr
+  | (ToServer c _ | FromServer c _) :: tr =>
+    is_open c /\ open_trace is_open tr
+  end.
+
+Lemma open_trace_prop {byte'}
+           (is_open is_open' : _) (tr : list (event byte')) :
+  open_trace is_open tr ->
+  (forall c, is_open c <-> is_open' c) ->
+  open_trace is_open' tr.
+Proof.
+  generalize dependent is_open.
+  generalize dependent is_open'.
+  induction tr as [ | [ c | c b | c b] tr ];
+    intros is_open is_open' Htr_open Hopen.
+  - auto.
+  - split.
+    + rewrite <- Hopen.
+      apply Htr_open.
+    + eapply IHtr.
+      { apply Htr_open. }
+      { intro c0.
+        split; intros [Hc0 | Hc0];
+          auto;
+          right; apply Hopen; auto.
+      }
+  - split.
+    + rewrite <- Hopen.
+      apply Htr_open.
+    + eapply IHtr.
+      { apply Htr_open. }
+      auto.
+  - split.
+    + rewrite <- Hopen.
+      apply Htr_open.
+    + eapply IHtr.
+      { apply Htr_open. }
+      auto.
+Qed.
+
+Axiom equiv_open_wf :
+  forall {byte'} (tr : list (event byte')),
+    open_trace (fun _ => False) tr <-> wf_trace tr.
+
+Lemma scrambled_preserves_wf : forall tr str : real_trace,
+    wf_trace tr ->
+    network_scrambled0 tr str ->
+    wf_trace str.
+Proof.
+Admitted.
+
+Definition network_scrambled_wf ns (tr0 tr1 : real_trace) :=
+  wf_trace tr0 ->
+  wf_trace tr1 ->
+  network_scrambled ns tr0 tr1.
+
+Definition network_scrambled_wf0 := network_scrambled_wf initial_ns.
+
+(* TODO: we can always append ServerSend and ClientSend
+   and preserve the [network_scrambled] property. *)
+
+Definition combined_networks (ns01 ns12 ns02 : network_state) : Prop :=
+  forall c,
+    let cs01 := Map.lookup ns01 c in
+    let cs12 := Map.lookup ns12 c in
+    let cs02 := Map.lookup ns02 c in
+    match connection_status cs01, connection_status cs12 with
+    | CLOSED, CLOSED => connection_status cs01 = CLOSED
+    | CLOSED, PENDING
+    | PENDING, PENDING =>
+      connection_status cs01 = PENDING
+    | ACCEPTED, PENDING
+    | ACCEPTED, ACCEPTED =>
+      connection_status cs01 = ACCEPTED
+    | CLOSED, ACCEPTED
+    | PENDING, ACCEPTED
+    | ACCEPTED, CLOSED
+    | PENDING, CLOSED => False
+    end /\
+    connection_inbytes cs01 ++ connection_inbytes cs12
+    = connection_inbytes cs02 /\
+    connection_outbytes cs12 ++ connection_outbytes cs01
+    = connection_outbytes cs02.
+
+Lemma scrambled_transitive_empty
+      (ns12 ns02 ns01 : network_state) tr2 :
+  combined_networks ns01 ns12 ns02 ->
+  network_scrambled ns12 [] tr2 ->
+  network_scrambled ns02 [] tr2.
+Proof.
+Admitted.
+
+Lemma scrambled_transitive_ ns01 ns12 ns02 tr0 tr1 tr2 :
+  combined_networks ns01 ns12 ns02 ->
+  network_scrambled ns01 tr0 tr1 ->
+  network_scrambled ns12 tr1 tr2 ->
+  network_scrambled ns02 tr0 tr2.
+Proof.
+  intros Hcombined H01_scrambled.
+  generalize dependent tr2.
+  generalize dependent Hcombined.
+  induction H01_scrambled;
+    intros.
+  - eapply scrambled_transitive_empty; eauto.
+  - econstructor.
+
+(*
+Lemma scrambled_transitive_
+*)
+
+Admitted.
+
+Instance scrambled_transitive : Transitive network_scrambled0.
+Proof.
+  unfold Transitive.
+Admitted.
+
+(* The notion of "open" connection is not quite the same
+   depending on whether we're on the client side or server side. *)
+
+(* For a client, open connections are those that are
+   [PENDING] or [ACCEPTED]. *)
+Definition is_open_conns_client ns : connection_id -> Prop :=
+  fun c =>
+    connection_status (Map.lookup ns c)
+    <> CLOSED.
+
+(* For a server, open connections are those that it [ACCEPTED]. *)
+Definition is_open_conns_server ns : connection_id -> Prop :=
+  fun c =>
+    connection_status (Map.lookup ns c) = ACCEPTED.
+
+(* [clean_state ns] holds when all connections [ns]
+   have empty buffers. *)
+Definition clean_state (ns : network_state) := forall c,
+    let cs := Map.lookup ns c in
+    connection_status cs <> PENDING /\
+    connection_inbytes  cs = [] /\
+    connection_outbytes cs = [].
+
+(*
+Lemma connect_accept ns c c0 :
+  Map.lookup (unsafe_accept_ns (unsafe_connect_ns ns c) c) c0
+  = if c = c0 ? then
+      {| connection_status := ACCEPTED;
+         connection_inbytes := [];
+         connection_outbytes := []; |}
+    else
+      Map.lookup ns c0.
+Proof.
+Admitted.
+*)
+
+Definition bind_transition {S B}
+           (a : option (S * unit)) (b : S -> option (S * B)) :
+  option (S * B) :=
+  match a with
+  | Some (s, _) => b s
+  | None => None
+  end.
+
+Infix ">>=" := bind_transition (at level 30).
+
+Lemma direct_to_server ns c b :
+  connection_inbytes (Map.lookup ns c) = [] ->
+  (client_send c b ns >>= server_recv c) = Some (ns, b).
+Proof.
+  intro Hc.
+  simpl.
+  rewrite Hc.
+  unfold server_recv.
+  rewrite Map.update_lookup_eq by reflexivity.
+  simpl.
+  rewrite Map.update_update_eq by reflexivity.
+  erewrite Map.lookup_update_eq; eauto.
+  destruct Map.lookup.
+  unfold update_in; simpl.
+  f_equal; auto.
+Qed.
+
+Lemma direct_from_server ns c b :
+  connection_outbytes (Map.lookup ns c) = [] ->
+  server_send c b ns >>= client_recv c = Some (ns, b).
+Proof.
+  intro Hc.
+  simpl.
+  rewrite Hc.
+  unfold client_recv.
+  rewrite Map.update_lookup_eq by reflexivity.
+  simpl.
+  rewrite Map.update_update_eq by reflexivity.
+  erewrite Map.lookup_update_eq; eauto.
+  destruct Map.lookup.
+  unfold update_out; simpl.
+  f_equal; auto.
+Qed.
+
+Lemma open_scrambled_reflexive :
+  forall ns tr,
+    clean_state ns ->
+    open_trace (is_open_conns_server ns) tr ->
+    network_scrambled ns tr tr.
+Proof.
+  intros ns tr.
+  generalize dependent ns.
+  induction tr as [ | [ c | c b | c b ] tr ];
+    intros ns Hns_clean Htr_open.
+  - (* [] *) constructor.
+  - (* NewConnection c :: tr *)
+    eapply ScrambleClient.
+    { simpl. rewrite connect_success.
+      { reflexivity. }
+      { destruct Htr_open.
+        unfold is_open_conns_server in H.
+        destruct (Hns_clean c) as [ ? ? ].
+        destruct connection_status; auto.
+        exfalso; auto.
+        exfalso; auto. }
+    }
+    eapply ScrambleServer.
+    { simpl. rewrite accept_success.
+      { reflexivity. }
+      { destruct Htr_open.
+        unfold is_open_conns_server in H.
+        rewrite Map.update_lookup_eq; auto. }
+    }
+    apply IHtr.
+    + rewrite Map.update_update_eq by reflexivity.
+      rewrite Map.update_lookup_eq by reflexivity.
+      intro c0.
+      destruct (@dec (c = c0)).
+      { typeclasses eauto. }
+      { rewrite Map.update_lookup_eq by assumption.
+        simpl; split; auto; discriminate. }
+      { rewrite Map.update_lookup_neq by assumption.
+        apply Hns_clean. }
+    + destruct Htr_open as [Htr0 Htr1].
+      apply open_trace_prop with (1 := Htr1).
+      intros c0.
+      unfold is_open_conns_server.
+      rewrite Map.update_update_eq by reflexivity.
+      rewrite Map.update_lookup_eq with (1 := eq_refl).
+      destruct (@dec (c = c0)).
+      { typeclasses eauto. }
+      { rewrite Map.update_lookup_eq by assumption.
+        split; auto. }
+      { rewrite Map.update_lookup_neq by assumption.
+        split; auto.
+        intros []; auto; contradiction. }
+  - (* ToServer c b :: tr *)
+    eapply ScrambleClient.
+    { reflexivity. }
+    eapply ScrambleServer.
+    { simpl.
+      pose proof direct_to_server as H.
+      simpl in H.
+      rewrite H.
+      reflexivity.
+      apply Hns_clean. }
+    apply IHtr.
+    { auto. }
+    { apply Htr_open. }
+  - (* FromServer c b :: tr *)
+    eapply ScrambleServer.
+    { reflexivity. }
+    eapply ScrambleClient.
+    { simpl.
+      pose proof direct_from_server as H.
+      simpl in H.
+      rewrite H.
+      reflexivity.
+      apply Hns_clean. }
+    apply IHtr.
+    { auto. }
+    { apply Htr_open. }
+Qed.
+
+Instance scrambled_reflexive : Reflexive network_scrambled_wf0.
+Proof.
+  unfold Reflexive.
+  intros tr Htr_wf _H. clear _H.
+  apply equiv_open_wf in Htr_wf.
+  apply open_scrambled_reflexive.
+  { intro c; split; auto; discriminate. }
+  { apply open_trace_prop with (1 := Htr_wf).
+    unfold is_open_conns_server.
+    simpl.
+    split; discriminate + intros []. }
+Qed.
+
+End ScramblingFacts.
