dw/DeepWeb/Lib/SimpleSpec_Traces.v
@@ -1,0 +1,204 @@
+Require Import Relations.
+Require Import RelationClasses.
+
+From QuickChick Require Import QuickChick.
+From Custom Require Import List Show String.
+Import ListNotations.
+From Custom Require Map.
+
+Require Import DeepWeb.Free.Monad.Free.
+Require Import DeepWeb.Free.Monad.Common.
+Import NonDeterminismBis.
+Import SumNotations.
+
+Require Import DeepWeb.Lib.Util.
+Require Import DeepWeb.Lib.SimpleSpec_NetworkModel.
+
+Set Bullet Behavior "Strict Subproofs".
+
+(* An event can be observed to happen on the network,
+   either from the server's or the client's point of view.
+   It is paremeterized by the type to represent the server's
+   output... *)
+Inductive event (byte' : Type) :=
+| NewConnection : connection_id -> event byte'
+| ToServer : connection_id -> byte -> event byte'
+| FromServer : connection_id -> byte' -> event byte'
+.
+
+Arguments NewConnection {byte'}.
+Arguments ToServer {byte'}.
+Arguments FromServer {byte'}.
+
+(* ... In the real world, this output is a concrete byte. *)
+Definition real_event := event byte.
+
+(* ... but it will also be useful for testing to insert hypothetical
+   bytes of unknown values in a trace, representing values that the
+   server may have output but which have not reached the client yet. *)
+Definition hypo_event := event (option byte).
+
+Definition show_real_event (ev : real_event) :=
+  match ev with
+  | NewConnection c => (show c ++ " !")%string
+  | ToServer c b =>
+    (show c ++ " <-- """ ++ pretty_char b ++ """")%string
+  | FromServer c b =>
+    (show c ++ " --> " ++ pretty_char b ++ """")%string
+  end.
+
+Instance Show_real_event: Show real_event :=
+  { show := show_real_event }.
+
+Definition show_hypo_event (ev : hypo_event) :=
+  match ev with
+  | NewConnection c => (show c ++ " !")%string
+  | ToServer c b =>
+    (show c ++ " <-- """ ++ pretty_char b ++ """")%string
+  | FromServer c ob =>
+    (show c ++ " --> " ++ match ob with
+                          | Some b => pretty_char b
+                          | None => "?"
+                          end ++ """")%string
+  end.
+
+Instance Show_hypo_event: Show hypo_event :=
+  { show := show_hypo_event }.
+
+(* Lists of events are traces. Again, we have two kinds of traces
+   corresponding to the two kinds of events. *)
+Definition real_trace := list real_event.
+Definition hypo_trace := list hypo_event.
+
+(* We can convert real things to hypothetical things. *)
+
+Definition real_to_hypo_event : real_event -> hypo_event :=
+  fun ev =>
+    match ev with
+    | NewConnection c => NewConnection c
+    | ToServer c b => ToServer c b
+    | FromServer c b => FromServer c (Some b)
+    end.
+
+Coercion real_to_hypo_event : real_event >-> hypo_event.
+
+Definition real_to_hypo_trace : real_trace -> hypo_trace :=
+  map real_to_hypo_event.
+
+Coercion real_to_hypo_trace : real_trace >-> hypo_trace.
+
+(* We relate events to effects as follows: an event is a pair of
+   an effect (of type [eff X] for some [X]) and a result (of
+   type [X]). *)
+Class EventType (event : Type) (eff : Type -> Type) :=
+  Build_EventType {
+    from_event : event -> { X : Type & (eff X * X)%type };
+  }.
+
+Definition event_eff
+           {event} {eff} `{EventType event eff} (ev : event) :
+  eff (projT1 (from_event ev)) :=
+  fst (projT2 (from_event ev)).
+
+Definition event_res
+           {event} {eff} `{EventType event eff} (ev : event) :
+  projT1 (from_event ev) :=
+  snd (projT2 (from_event ev)).
+
+(* [E +' F] is a signature of _visible_ effects [F] and _invisible_
+   effects [E]. The trace (of type [list event]) is a sequence of
+   visible effects [F] with their results. *)
+Inductive is_trace
+          {event : Type} {E F : Type -> Type} {R : Type}
+          `{EventType event F} :
+  M (E +' F) R -> list event -> Prop :=
+| ServerEmpty : forall s, is_trace s []
+| ServerVis : forall ev k tr,
+    is_trace (k (event_res ev)) tr ->
+    is_trace (Vis (| event_eff ev) k) (ev :: tr)
+| ServerInvis : forall X e k (x : X) tr,
+    is_trace (k x) tr ->
+    is_trace (Vis (e |) k) tr
+.
+
+Definition server_transition (ev : real_event) :
+  network_state -> network_state -> Prop :=
+  fun ns ns' =>
+    match ev with
+    | NewConnection c => server_accept c ns = Some (ns', tt)
+    | ToServer c b => server_recv c ns = Some (ns', b)
+    | FromServer c b => server_send c b ns = Some (ns', tt)
+    end.
+
+Definition client_transition (ev : real_event) :
+  network_state -> network_state -> Prop :=
+  fun ns ns' =>
+    match ev with
+    | NewConnection c => client_connect c ns = Some (ns', tt)
+    | ToServer c b => client_send c b ns = Some (ns', tt)
+    | FromServer c b => client_recv c ns = Some (ns', b)
+    end.
+
+(* Corresponding "server-side" and "client-side" traces. *)
+Inductive network_scrambled :
+  network_state -> real_trace -> real_trace -> Prop :=
+| ScrambleEmpty : forall ns, network_scrambled ns [] []
+| ScrambleServer : forall ns ns' e tr_server tr_client,
+    server_transition e ns ns' ->
+    network_scrambled ns'       tr_server  tr_client ->
+    network_scrambled ns  (e :: tr_server) tr_client
+| ScrambleClient : forall ns ns' e tr_server tr_client,
+    client_transition e ns ns' ->
+    network_scrambled ns' tr_server       tr_client ->
+    network_scrambled ns  tr_server (e :: tr_client)
+.
+
+Definition network_scrambled0 := network_scrambled initial_ns.
+
+Definition event_connection {byte'} (ev : event byte') :
+  connection_id :=
+  match ev with
+  | NewConnection c' => c'
+  | ToServer c' _ => c'
+  | FromServer c' _ => c'
+  end.
+
+(* Some notations to make traces readable. *)
+Module EventNotations.
+Delimit Scope event_scope with event.
+
+(* Connection [c] is open. *)
+Notation "c !" := (NewConnection (Connection c))
+(at level 30) : real_scope.
+
+(* Byte [b] goes to the server on connection [c]. *)
+Notation "c <-- b" := (ToServer (Connection c) b%char)
+(at level 30) : real_scope.
+
+(* Byte [b] goes out of the server on connection [c]. *)
+Notation "c --> b" := (FromServer (Connection c) b%char)
+(at level 30) : real_scope.
+
+Notation "c !" := (NewConnection (Connection c) : event (option byte))
+(at level 30) : hypo_scope.
+
+(* Byte [b] goes to the server on connection [c]. *)
+Notation "c <-- b" :=
+  (ToServer (Connection c) b%char : event (option byte))
+(at level 30) : hypo_scope.
+
+(* Byte [b] goes out of the server on connection [c]. *)
+Notation "c --> b" :=
+  (FromServer (Connection c) (Some b)%char : event (option byte))
+(at level 30) : hypo_scope.
+
+(* Unknown byte goes out of the server on connection [c]. *)
+Notation "c --> ?" := (FromServer (Connection c) None : event (option byte))
+(at level 30) : hypo_scope.
+
+(* Open Scope real_scope. *)
+
+Delimit Scope hypo_scope with hypo.
+Delimit Scope real_scope with real.
+
+End EventNotations.
